examples/dm4free/ifc.fst
@@ -3,42 +3,45 @@ module IFC
 (********************************************************************************)
 (* Effect (ifc a) : A monad for dynamic information-flow control                *)
 (********************************************************************************)
+
+(* TODO: This has not been whitelisted
 type label =
   | Low
   | High
+*)
+type label = bool
+inline let low = true
+inline let high = false
+
+(* working around the whitelist *)
+inline let eq l1 l2 =
+  match l1, l2 with
+  | true, true
+  | false, false -> true
+  | _, _ -> false
 
 let join l1 l2 =
-  match l1, l2 with
-  | _   , High
-  | High, _    -> High
-  | _   , _    -> Low
+  if l1 `eq` high || l2 `eq` high then high else low
 
-let flows l1 l2 =
-  match l1, l2 with
-  | High, Low -> false
-  | _   , _   -> true
+let flows l1 l2 = not(l1 `eq` high && l2 `eq` low)
 
-type err (a:Type) =
-  | Leak 
-  | Result : v:a -> err a
-
-let ifc (a:Type) = label -> Tot (err (a * label))
+let ifc (a:Type) = label -> Tot (option (a * label))
 
 (* open FStar.FunctionalExtensionality *)
 
 let eq_ifc (a:Type) (f:ifc a) (g:ifc a) =
    forall l. f l == g l
 
-let return_ifc (a:Type) (x:a) : ifc a = fun l -> Result (x, l)
-let bind_ifc (a:Type) (b:Type) (f:ifc a) (g: a -> Tot (ifc b)) : ifc b 
-  = fun l0 -> match f l0 with 
-	   | Leak -> Leak
-	   | Result (x, l1) -> 
+let return_ifc (a:Type) (x:a) : ifc a = fun l -> Some (x, l)
+let bind_ifc (a:Type) (b:Type) (f:ifc a) (g: a -> Tot (ifc b)) : ifc b
+  = fun l0 -> match f l0 with
+	   | None -> None
+	   | Some (x, l1) ->
 	     match g x l1 with
-	     | Leak -> Leak
-	     | Result (y, l2) -> Result(y, l2)
+	     | None -> None
+	     | Some (y, l2) -> Some(y, l2)
 
-val left_unit: a:Type -> b:Type -> x:a -> f:(a -> Tot (ifc b)) 
+val left_unit: a:Type -> b:Type -> x:a -> f:(a -> Tot (ifc b))
 	    -> Lemma (eq_ifc b (bind_ifc a b (return_ifc a x) f) (f x))
 let left_unit a b x f = ()
 
@@ -47,25 +50,39 @@ let right_unit a f = ()
 
 val associativity: a:Type -> b:Type -> c:Type -> f:ifc a -> g:(a -> Tot (ifc b)) -> h:(b -> Tot (ifc c))
 		 -> Lemma (eq_ifc c (bind_ifc a c f (fun x -> bind_ifc b c (g x) h)) (bind_ifc b c (bind_ifc a b f g) h))
-let associativity a b c f g h = ()		 
+let associativity a b c f g h = ()
 
 // Some dummy implementations of actions for illustration purposes
 // Probably better to just take them axiomatically
-let read (l:label) : ifc bool = fun l0 -> Result (true, join l0 l)
+let read (l:label) : ifc bool = fun l0 -> Some (true, join l0 l)
 let write (l:label) (b:bool) : ifc unit =
-  fun l0 -> if flows l0 l then (Result ((), l0)) else Leak
+  fun l0 -> if flows l0 l then (Some ((), l0)) else None
 
 let xor (b1:bool) (b2:bool) : Tot bool = not (b1 = b2)
 
 // A sample monadic program (normally would write this after
 // elaboration, but whatever, can write this in DM too)
-val p : unit -> Pure (ifc unit) (requires True) (ensures (fun r -> forall l. r l = Leak))
+val p : unit -> Pure (ifc unit) (requires True) (ensures (fun r -> forall l. r l = None))
 (* Weak type (works): unit -> Tot (ifc unit) *)
 (* Alternative strong type (doesn't work), (Valid(ApplyTT@2 @0))
-  unit -> Tot (label -> Pure (err (unit * label)) (requires True) (ensures (fun r -> r = Leak))) *)
-let p () = bind_ifc _ _ (read Low)              (fun b1 ->
-           bind_ifc _ _ (read Low)              (fun b2 ->
-           bind_ifc _ _ (write Low (b1 && b2))  (fun _  ->
-           bind_ifc _ _ (read High)             (fun b3 ->
-           bind_ifc _ _ (write High (b1 || b3)) (fun _  ->
-                        (write Low (xor b3 b3))  )))))
+  unit -> Tot (label -> Pure (err (unit * label)) (requires True) (ensures (fun r -> r = None))) *)
+let p () = bind_ifc _ _ (read low)              (fun b1 ->
+           bind_ifc _ _ (read low)              (fun b2 ->
+           bind_ifc _ _ (write low (b1 && b2))  (fun _  ->
+           bind_ifc _ _ (read high)             (fun b3 ->
+           bind_ifc _ _ (write high (b1 || b3)) (fun _  ->
+                        (write low (xor b3 b3))  )))))
+
+new_effect_for_free {
+  ExnState : a:Type -> Effect
+  with
+       repr         = ifc
+     ; bind         = bind_ifc
+     ; return       = return_ifc
+  and effect_actions
+      read = read
+    ; write = write
+}
+(* TODO: make this work *)
+(* Error: Unexpected error; please file a bug report, ideally with a minimized version of the source program that triggered the error. *)
+(* Failure("not a C") *)
